simplify proofs

FOL.v
@@ -13,7 +13,7 @@ Notation "∀ p ":= (All_ _ _ p) (at level 60).
 Section implicative.
 
   Variable form : Type.
-  Variable retract_implicative : retract (form_implicative form) form.
+  Variable retract_implicative : included form_implicative form.
 
   Variable count : form -> nat.
   Definition count_imp (p : form_implicative form) := match p with
@@ -24,37 +24,38 @@ Section implicative.
 
   Variable nd : list form -> form -> Prop.
   Notation "A ⊢ p" := (nd A p) (at level 70).
+  Variable ndH : forall A p, In p A -> A ⊢ p.
+
   Inductive nd_imp (A : list form) : form -> Prop :=
-    | ndHI p : In p A -> A ⊢I p
+    | ndHI p : A ⊢ p -> A ⊢I p
     | ndExp p : A ⊢ ⊥ -> A ⊢I p
     | ndII p q : (p :: A) ⊢ q -> A ⊢I p ~> q
     | ndIE p q : A ⊢ p ~> q -> A ⊢ p -> A ⊢I q
   where "A ⊢I p" := (nd_imp A p).
 
+  Variable agree : forall A p, A ⊢I p -> A ⊢ p.
+
   Variable weakening : forall A B p, A ⊢ p -> incl A B -> B ⊢ p.
   Lemma weakening_imp A B p : A ⊢I p -> incl A B -> B ⊢I p.
-  Proof. intro. revert B. induction H; intros B Hinc.
-    -apply ndHI. now apply Hinc.
-    -apply ndExp. now apply (weakening A).
-    -apply ndII. apply (weakening (p::A) (p::B)). assumption. { apply incl_cons. now left. now apply incl_tl. }
-    -apply (ndIE _ p). now apply (weakening A B (p~>q)). now apply (weakening A).
+  Proof. intro. revert B. induction H; intros B Hinc;
+    [ apply ndHI | apply ndExp | apply ndII | apply (ndIE _ p _ (weakening _ _ _ H Hinc)) ].
+    1,2,4: now apply (weakening A).
+    apply (weakening (p::A) (p::B) _ H), incl_cons; [ now left | now apply incl_tl ].
   Qed.
 
+  Variable retract : included form_implicative (form_implicative form).
   Variable translate : form -> form.
-  Definition translate_imp (p : form_implicative form) := match p with
-    | Fal _ => Impl _ (¬⊥) (⊥)
+  Definition translate_imp (p : form_implicative form) : form_implicative form := match p with
+    | Fal _ => ¬¬⊥
     | Impl _ p q => Impl _ (translate p) (translate q)
   end.
 
-  Variable agree : forall A p, nd A p <-> A ⊢I p.
   Variable double_neg : forall A p, A ⊢ p -> A ⊢ translate p.
-  Lemma double_neg_imp A p : A ⊢I p -> A ⊢I translate p.
-  Proof. induction 1; apply agree, double_neg, agree.
-    -now apply ndHI.
-    -now apply ndExp.
-    -now apply ndII.
-    -now apply (ndIE _ p).
+  Lemma double_neg_imp A p : A ⊢I p -> A ⊢I (translate p).
+  Proof. induction 1; apply ndHI, double_neg, agree;
+    [ now apply ndHI | now apply ndExp | now apply ndII | now apply (ndIE _ p) ].
   Qed.
+
 End implicative.
 
 Section universals.
@@ -71,35 +72,39 @@ Section universals.
 
   Variable nd : list form -> form -> Prop.
   Notation "A ⊢ p" := (nd A p) (at level 70).
+  Variable ndH : forall A p, In p A -> A ⊢ p.
+
   Definition up_ctx (A : list form) := map (subst_form (S >> var_term)) A.
   Inductive nd_univ (A : list form) : form -> Prop :=
+    | ndHU p : A ⊢ p -> A ⊢U p
     | ndUI p : up_ctx A ⊢ p -> A ⊢U ∀ p
     | ndUE p t : A ⊢ ∀ p -> A ⊢U subst_form (t ..) p
   where "A ⊢U p" := (nd_univ A p).
 
+  Variable agree : forall A p, A ⊢U p -> A ⊢ p.
 
   Variable weakening : forall A B p, A ⊢ p -> incl A B -> B ⊢ p.
   Lemma weakening_univ A B p : A ⊢U p -> incl A B -> B ⊢U p.
-  Proof. intro. revert B. induction H; intros B Hinc.
-    -apply ndUI. apply (weakening (up_ctx A) (up_ctx B)). assumption. unfold up_ctx. now apply incl_map.
-    -apply ndUE. now apply (weakening A).
+  Proof. intro. revert B. induction H; intros B Hinc; [ apply ndHU | apply ndUI | apply ndUE ].
+    1,3: now apply (weakening A).
+    -apply (weakening (up_ctx A) (up_ctx B)); [ assumption | unfold up_ctx ]. now apply incl_map.
   Qed.
 
 
-  Variable retract_implicative : retract (form_implicative form) form.
-  Variable retract_imp2univ : retract (form_implicative (form_univ form)) (form_univ form).
+  Variable retract_implicative : included form_implicative form.
+  Variable retract_imp_univ : included form_implicative (form_univ form).
+
   Variable translate : form -> form.
-  Definition translate_univ (p : form_univ form) : form_univ form := match p with
+  Definition translate_univ (p : form_univ form) : _ := match p with
     | Pred _ _ _ => ¬¬p
-    | All _ f => All _ (translate f)
+    | All _ q => All _ (translate q)
   end.
 
-  Variable agree : forall A p, nd A p <-> A ⊢U p.
   Variable double_neg : forall A p, A ⊢ p -> A ⊢ translate p.
+
   Lemma double_neg_univ A p : A ⊢U p -> A ⊢U translate p.
-  Proof. induction 1; apply agree, double_neg, agree.
-    -now apply ndUI.
-    -now apply ndUE.
+  Proof. induction 1; apply ndHU, double_neg, agree;
+    [ now apply ndHU | now apply ndUI | now apply ndUE ].
   Qed.
 
 End universals.
@@ -114,26 +119,25 @@ Inductive nd : list form -> form -> Prop :=
   | ndU A p : nd_univ form _ subst_form nd A p -> A ⊢ p
 where "A ⊢ p" := (nd A p).
 
-(* Fixpoint weakening A B p: A ⊢ p -> incl A B -> B ⊢ p.
-Proof. destruct 1; intro Hinc.
-    -apply ndI. now apply (weakening_imp _ _ nd weakening A B).
-    -apply ndU. now apply (weakening_univ _ _ subst_form nd weakening A B).
+(* Fixpoint weakening A B p : A ⊢ p -> incl A B -> B ⊢ p.
+Proof. destruct 1; intro Hinc; [ apply ndI | apply ndU ].
+    -now apply (weakening_imp form _ nd weakening A B).
+    -now apply (weakening_univ form _ subst_form nd weakening A B).
 Qed. *)
 
+Section double_neg.
+  Variable retract_imp2imp : included form_implicative (form_implicative form).
+  Variable retract_imp2univ : included form_implicative (form_univ form).
 
-Variable retract_imp2univ : retract (form_implicative (form_univ form)) (form_univ form).
-Fixpoint translate (p : form) := match p with
-  | In_form_implicative p => inj (translate_imp form _ translate p)
-  | In_form_univ p => inj (translate_univ form retract_imp2univ translate p)
-end.
+  Fixpoint translate (p : form) : form := match p with
+    | In_form_implicative p => inj (translate_imp form _ translate p)
+    | In_form_univ p => inj (translate_univ form _ translate p)
+  end.
 
+(*  Fixpoint double_neg A p: A ⊢ p -> A ⊢ translate p.
+  Proof. destruct 1.
+    -apply ndI. now apply (double_neg_imp _ _ nd ndI translate double_neg).
+    -apply ndU. now apply (double_neg_univ _ _ subst_form nd ndU translate double_neg).
+  Qed. *)
 
-Variable agreeI : forall A p, nd A p <-> nd_imp _ _ nd A p.
-Variable agreeU : forall A p, nd A p <-> nd_univ _ _ subst_form nd A p.
-
-(* Fixpoint double_neg A p: A ⊢ p -> A ⊢ translate p.
-Proof. destruct 1.
-  -apply ndI. now apply (double_neg_imp _ _ nd translate agreeI double_neg).
-  -apply ndU. now apply (double_neg_univ _ _ subst_form nd translate agreeU double_neg).
-Qed. *)
-
+End double_neg.
